finish AsyncBlockCache

disk-betree/AsyncBlockCache.dfy
@@ -51,9 +51,45 @@ abstract module AsyncBlockCache refines Transactable {
   {
     ref in s.ephemeralIndirectionTable.graph
   }
-  predicate ValidLBAForNode(k: Constants, lba: LBA)
+  predicate ValidLBAForNode(lba: LBA)
   {
     lba != IndirectionTableLBA()
+  }
+
+  predicate method GraphClosed(graph: map<Reference, seq<Reference>>)
+  {
+    forall ref | ref in graph ::
+      forall succ | succ in graph[ref] ::
+        succ in graph
+  }
+
+  // WF IndirectionTable which must have all LBAs filled in
+  predicate WFCompleteIndirectionTable(indirectionTable: IndirectionTable)
+  {
+    && IndirectionTableLBA() !in indirectionTable.lbas.Values
+    && indirectionTable.graph.Keys == indirectionTable.lbas.Keys
+    && G.Root() in indirectionTable.graph
+    && GraphClosed(indirectionTable.graph)
+  }
+
+  // WF IndirectionTable which might not have all LBAs filled in
+  predicate WFIndirectionTable(k: Constants, indirectionTable: IndirectionTable)
+  {
+    && IndirectionTableLBA() !in indirectionTable.lbas.Values
+    && indirectionTable.lbas.Keys <= indirectionTable.graph.Keys
+    && G.Root() in indirectionTable.graph
+    && GraphClosed(indirectionTable.graph)
+  }
+
+  predicate LBAFree(s: Variables, lba: LBA)
+  requires s.Ready?
+  {
+    && lba !in s.persistentIndirectionTable.lbas.Values
+    && lba !in s.ephemeralIndirectionTable.lbas.Values
+    && (s.outstandingIndirectionTableWrite.Some? ==>
+        lba !in s.outstandingIndirectionTableWrite.value.indirectionTable.lbas.Values)
+    && (forall id | id in s.outstandingBlockWrites ::
+        s.outstandingBlockWrites[id].lba != lba)
   }
 
   datatype Step =
@@ -72,12 +108,11 @@ abstract module AsyncBlockCache refines Transactable {
 
   predicate WriteBackReq(k: Constants, s: Variables, s': Variables, dop: DiskOp, ref: Reference)
   {
-    && s.Ready?
     && dop.ReqWriteOp?
+    && s.Ready?
     && ref in s.cache
-    && ValidLBAForNode(k, dop.reqWrite.lba)
-    && dop.reqWrite.lba !in s.persistentIndirectionTable.lbas.Values
-    && dop.reqWrite.lba !in s.ephemeralIndirectionTable.lbas.Values
+    && ValidLBAForNode(dop.reqWrite.lba)
+    && LBAFree(s, dop.reqWrite.lba)
     && dop.reqWrite.sector == SectorBlock(s.cache[ref])
     && s'.Ready?
     && s'.persistentIndirectionTable == s.persistentIndirectionTable
@@ -87,21 +122,21 @@ abstract module AsyncBlockCache refines Transactable {
     && s'.outstandingBlockWrites == s.outstandingBlockWrites[dop.id := OutstandingWrite(ref, dop.reqWrite.lba)]
     && s'.outstandingBlockReads == s.outstandingBlockReads
     && s'.outstandingIndirectionTableWrite == s'.outstandingIndirectionTableWrite
-    && s.outstandingIndirectionTableWrite == s.outstandingIndirectionTableWrite
+    && s'.outstandingIndirectionTableWrite == s.outstandingIndirectionTableWrite
   }
 
   predicate WriteBackResp(k: Constants, s: Variables, s': Variables, dop: DiskOp)
   {
-    && s.Ready?
     && dop.RespWriteOp?
+    && s.Ready?
     && dop.id in s.outstandingBlockWrites
     && s' == s.(outstandingBlockWrites := MapRemove1(s.outstandingBlockWrites, dop.id))
   }
 
   predicate WriteBackIndirectionTableReq(k: Constants, s: Variables, s': Variables, dop: DiskOp)
   {
-    && s.Ready?
     && dop.ReqWriteOp?
+    && s.Ready?
     && dop.reqWrite.lba == IndirectionTableLBA()
     && dop.reqWrite.sector == SectorIndirectionTable(s.ephemeralIndirectionTable)
     && s.cache.Keys <= s.ephemeralIndirectionTable.lbas.Keys
@@ -112,8 +147,8 @@ abstract module AsyncBlockCache refines Transactable {
 
   predicate WriteBackIndirectionTableResp(k: Constants, s: Variables, s': Variables, dop: DiskOp)
   {
-    && s.Ready?
     && dop.RespWriteOp?
+    && s.Ready?
     && s.outstandingIndirectionTableWrite.Some?
     && dop.id == s.outstandingIndirectionTableWrite.value.reqId
     && s' == s.(outstandingIndirectionTableWrite := None)
@@ -127,8 +162,8 @@ abstract module AsyncBlockCache refines Transactable {
 
   predicate Unalloc(k: Constants, s: Variables, s': Variables, dop: DiskOp, ref: Reference)
   {
-    && s.Ready?
     && dop.NoDiskOp?
+    && s.Ready?
 
     && IsAllocated(s, ref)
 
@@ -141,17 +176,376 @@ abstract module AsyncBlockCache refines Transactable {
     && s'.ephemeralIndirectionTable.lbas == MapRemove(s.ephemeralIndirectionTable.lbas, {ref})
     && s'.cache == MapRemove(s.cache, {ref})
     && s'.ephemeralIndirectionTable.graph == MapRemove(s.ephemeralIndirectionTable.graph, {ref})
+
+    && s'.outstandingIndirectionTableWrite == s.outstandingIndirectionTableWrite
+    && s'.outstandingBlockWrites == s.outstandingBlockWrites
+    && s'.outstandingBlockReads == s.outstandingBlockReads
   }
 
   predicate PageInReq(k: Constants, s: Variables, s': Variables, dop: DiskOp, ref: Reference)
   {
-    && s.Ready?
     && dop.ReqReadOp?
+    && s.Ready?
     && IsAllocated(s, ref)
     && ref in s.ephemeralIndirectionTable.lbas
     && ref !in s.cache
     && s.ephemeralIndirectionTable.lbas[ref] == dop.reqRead.lba
     && s' == s.(outstandingBlockReads := s.outstandingBlockReads[dop.id := OutstandingRead(ref)])
   }
+
+  predicate PageInResp(k: Constants, s: Variables, s': Variables, dop: DiskOp)
+  {
+    && dop.RespReadOp?
+    && s.Ready?
+    && dop.id in s.outstandingBlockReads
+    && var ref := s.outstandingBlockReads[dop.id].ref;
+    && ref !in s.cache
+    && dop.respRead.sector.SectorBlock?
+    && var block := dop.respRead.sector.block;
+    && ref in s.ephemeralIndirectionTable.graph
+    && (iset r | r in s.ephemeralIndirectionTable.graph[ref]) == G.Successors(block)
+    && s' == s.(cache := s.cache[ref := block])
+              .(outstandingBlockReads := MapRemove1(s.outstandingBlockReads, dop.id))
+  }
+
+  predicate PageInIndirectionTableReq(k: Constants, s: Variables, s': Variables, dop: DiskOp)
+  {
+    && dop.ReqReadOp?
+    && s.Unready?
+    && s.outstandingIndirectionTableRead.None?
+    && dop.reqRead.lba == IndirectionTableLBA()
+    && s' == Unready(Some(dop.id))
+  }
+
+  predicate PageInIndirectionTableResp(k: Constants, s: Variables, s': Variables, dop: DiskOp)
+  {
+    && dop.RespReadOp?
+    && s.Unready?
+    && s.outstandingIndirectionTableRead == Some(dop.id)
+    && dop.respRead.sector.SectorIndirectionTable?
+    && WFCompleteIndirectionTable(dop.respRead.sector.indirectionTable)
+    && s' == Ready(dop.respRead.sector.indirectionTable, dop.respRead.sector.indirectionTable, None, map[], map[], map[])
+  }
+
+  predicate Evict(k: Constants, s: Variables, s': Variables, dop: DiskOp, ref: Reference)
+  {
+    && s.Ready?
+    && dop.NoDiskOp?
+    && ref in s.cache
+    && ref in s.ephemeralIndirectionTable.lbas
+    && OutstandingWrite(ref, s.ephemeralIndirectionTable.lbas[ref]) !in s.outstandingBlockWrites.Values
+    && s' == s.(cache := MapRemove(s.cache, {ref}))
+  }
+
+  predicate NoOp(k: Constants, s: Variables, s': Variables, dop: DiskOp)
+  {
+    && (dop.RespReadOp? || dop.NoDiskOp?)
+    && s' == s
+  }
+
+  ////// Write/Alloc Ops
+
+  predicate BlockPointsToValidReferences(block: Node, graph: map<Reference, seq<Reference>>)
+  {
+    forall ref | ref in G.Successors(block) :: ref in graph
+  }
+
+  predicate Dirty(k: Constants, s: Variables, s': Variables, ref: Reference, block: Node)
+  {
+    // Possibly allocs ref, possibly overwrites it.
+    && s.Ready?
+    && ref in s.cache
+    && s'.Ready?
+    && s'.cache == s.cache[ref := block]
+    && s'.persistentIndirectionTable == s.persistentIndirectionTable
+
+    && s'.ephemeralIndirectionTable.lbas == MapRemove(s.ephemeralIndirectionTable.lbas, {ref})
+
+    && BlockPointsToValidReferences(block, s.ephemeralIndirectionTable.graph)
+
+    && ref in s'.ephemeralIndirectionTable.graph
+    && s'.ephemeralIndirectionTable.graph == s.ephemeralIndirectionTable.graph[ref := s'.ephemeralIndirectionTable.graph[ref]]
+    && (iset r | r in s'.ephemeralIndirectionTable.graph[ref]) == G.Successors(block)
+
+    && s'.outstandingIndirectionTableWrite == s.outstandingIndirectionTableWrite
+    && s'.outstandingBlockWrites == s.outstandingBlockWrites
+    && s'.outstandingBlockReads == s.outstandingBlockReads
+  }
+
+  predicate Alloc(k: Constants, s: Variables, s': Variables, ref: Reference, block: Node)
+  {
+    // Possibly allocs ref, possibly overwrites it.
+    && s.Ready?
+    && ref !in s.cache
+    && !IsAllocated(s, ref)
+    && s'.Ready?
+    && s'.cache == s.cache[ref := block]
+    && s'.persistentIndirectionTable == s.persistentIndirectionTable
+
+    && s'.ephemeralIndirectionTable.lbas == s.ephemeralIndirectionTable.lbas
+
+    && BlockPointsToValidReferences(block, s.ephemeralIndirectionTable.graph)
+
+    && ref in s'.ephemeralIndirectionTable.graph
+    && s'.ephemeralIndirectionTable.graph == s.ephemeralIndirectionTable.graph[ref := s'.ephemeralIndirectionTable.graph[ref]]
+    && (iset r | r in s'.ephemeralIndirectionTable.graph[ref]) == G.Successors(block)
+
+    && s'.outstandingIndirectionTableWrite == s.outstandingIndirectionTableWrite
+    && s'.outstandingBlockWrites == s.outstandingBlockWrites
+    && s'.outstandingBlockReads == s.outstandingBlockReads
+  }
+
+  predicate ReadStep(k: Constants, s: Variables, op: ReadOp)
+  {
+    s.Ready? && MapsTo(s.cache, op.ref, op.node)
+  }
+
+  predicate OpStep(k: Constants, s: Variables, s': Variables, op: Op)
+  {
+    match op {
+      case WriteOp(ref, block) => Dirty(k, s, s', ref, block)
+      case AllocOp(ref, block) => Alloc(k, s, s', ref, block)
+    }
+  }
+
+  predicate Transaction(k: Constants, s: Variables, s': Variables, dop: DiskOp, ops: seq<Op>)
+  {
+    && dop.NoDiskOp?
+    && OpTransaction(k, s, s', ops)
+  }
+
+  predicate Init(k: Constants, s: Variables)
+  {
+    s == Unready(None)
+  }
+
+  predicate NextStep(k: Constants, s: Variables, s': Variables, dop: DiskOp, step: Step) {
+    match step {
+      case WriteBackReqStep(ref) => WriteBackReq(k, s, s', dop, ref)
+      case WriteBackRespStep => WriteBackResp(k, s, s', dop)
+      case WriteBackIndirectionTableReqStep => WriteBackIndirectionTableReq(k, s, s', dop)
+      case WriteBackIndirectionTableRespStep => WriteBackIndirectionTableResp(k, s, s', dop)
+      case UnallocStep(ref) => Unalloc(k, s, s', dop, ref)
+      case PageInReqStep(ref) => PageInReq(k, s, s', dop, ref)
+      case PageInRespStep => PageInResp(k, s, s', dop)
+      case PageInIndirectionTableReqStep => PageInIndirectionTableReq(k, s, s', dop)
+      case PageInIndirectionTableRespStep => PageInIndirectionTableResp(k, s, s', dop)
+      case EvictStep(ref) => Evict(k, s, s', dop, ref)
+      case NoOpStep => NoOp(k, s, s', dop)
+      case TransactionStep(ops) => Transaction(k, s, s', dop, ops)
+    }
+  }
+
+  predicate Next(k: Constants, s: Variables, s': Variables, dop: DiskOp) {
+    exists step: Step :: NextStep(k, s, s', dop, step)
+  }
+
+  predicate CacheConsistentWithSuccessors(cache: map<Reference, Node>, graph: map<Reference, seq<Reference>>)
+  requires cache.Keys <= graph.Keys
+  {
+    forall ref | ref in cache :: (iset r | r in graph[ref]) == G.Successors(cache[ref])
+  }
+
+  predicate InvReady(k: Constants, s: Variables)
+  requires s.Ready?
+  {
+    && WFCompleteIndirectionTable(s.persistentIndirectionTable)
+    && WFIndirectionTable(k, s.ephemeralIndirectionTable)
+    && (s.outstandingIndirectionTableWrite.Some? ==>
+        WFCompleteIndirectionTable(s.outstandingIndirectionTableWrite.value.indirectionTable))
+    && s.cache.Keys <= s.ephemeralIndirectionTable.graph.Keys
+    && s.ephemeralIndirectionTable.graph.Keys <= s.cache.Keys + s.ephemeralIndirectionTable.lbas.Keys
+    && CacheConsistentWithSuccessors(s.cache, s.ephemeralIndirectionTable.graph)
+    && GraphClosed(s.ephemeralIndirectionTable.graph)
+  }
+
+  predicate Inv(k: Constants, s: Variables)
+  {
+    s.Ready? ==> InvReady(k, s)
+  }
+
+  lemma InitImpliesInv(k: Constants, s: Variables)
+    requires Init(k, s)
+    ensures Inv(k, s)
+  {
+  }
+
+  lemma WriteBackReqStepPreservesInv(k: Constants, s: Variables, s': Variables, dop: DiskOp, ref: Reference)
+    requires Inv(k, s)
+    requires WriteBackReq(k, s, s', dop, ref)
+    ensures Inv(k, s')
+  {
+    if (s'.Ready?) {
+      assert InvReady(k, s');
+    }
+  }
+
+  lemma WriteBackRespStepPreservesInv(k: Constants, s: Variables, s': Variables, dop: DiskOp)
+    requires Inv(k, s)
+    requires WriteBackResp(k, s, s', dop)
+    ensures Inv(k, s')
+  {
+    if (s'.Ready?) {
+      assert InvReady(k, s');
+    }
+  }
+
+  lemma WriteBackIndirectionTableReqStepPreservesInv(k: Constants, s: Variables, s': Variables, dop: DiskOp)
+    requires Inv(k, s)
+    requires WriteBackIndirectionTableReq(k, s, s', dop)
+    ensures Inv(k, s')
+  {
+    if (s'.Ready?) {
+      assert InvReady(k, s');
+    }
+  }
+
+  lemma WriteBackIndirectionTableRespStepPreservesInv(k: Constants, s: Variables, s': Variables, dop: DiskOp)
+    requires Inv(k, s)
+    requires WriteBackIndirectionTableResp(k, s, s', dop)
+    ensures Inv(k, s')
+  {
+    if (s'.Ready?) {
+      assert InvReady(k, s');
+    }
+  }
+
+  lemma DirtyStepPreservesInv(k: Constants, s: Variables, s': Variables, ref: Reference, block: Node)
+    requires Inv(k, s)
+    requires Dirty(k, s, s', ref, block)
+    ensures Inv(k, s')
+  {
+    if (s'.Ready?) {
+      assert InvReady(k, s');
+    }
+  }
+
+  lemma AllocStepPreservesInv(k: Constants, s: Variables, s': Variables, ref: Reference, block: Node)
+    requires Inv(k, s)
+    requires Alloc(k, s, s', ref, block)
+    ensures Inv(k, s')
+  {
+    if (s'.Ready?) {
+      assert InvReady(k, s');
+    }
+  }
+
+  lemma OpPreservesInv(k: Constants, s: Variables, s': Variables, op: Op)
+    requires Inv(k, s)
+    requires OpStep(k, s, s', op)
+    ensures Inv(k, s')
+  {
+    match op {
+      case WriteOp(ref, block) => DirtyStepPreservesInv(k, s, s', ref, block);
+      case AllocOp(ref, block) => AllocStepPreservesInv(k, s, s', ref, block);
+    }
+  }
+
+  lemma TransactionStepPreservesInv(k: Constants, s: Variables, s': Variables, dop: DiskOp, ops: seq<Op>)
+    requires Inv(k, s)
+    requires Transaction(k, s, s', dop, ops)
+    ensures Inv(k, s')
+    decreases |ops|
+  {
+    if (|ops| == 0) {
+    } else if (|ops| == 1) {
+      OpPreservesInv(k, s, s', ops[0]);
+    } else {
+      var ops1, smid, ops2 := SplitTransaction(k, s, s', ops);
+      TransactionStepPreservesInv(k, s, smid, dop, ops1);
+      TransactionStepPreservesInv(k, smid, s', dop, ops2);
+    }
+  }
+
+  lemma UnallocStepPreservesInv(k: Constants, s: Variables, s': Variables, dop: DiskOp, ref: Reference)
+    requires Inv(k, s)
+    requires Unalloc(k, s, s', dop, ref)
+    ensures Inv(k, s')
+  {
+    if (s'.Ready?) {
+      assert InvReady(k, s');
+    }
+  }
+
+  lemma PageInReqStepPreservesInv(k: Constants, s: Variables, s': Variables, dop: DiskOp, ref: Reference)
+    requires Inv(k, s)
+    requires PageInReq(k, s, s', dop, ref)
+    ensures Inv(k, s')
+  {
+    if (s'.Ready?) {
+      assert InvReady(k, s');
+    }
+  }
+
+  lemma PageInRespStepPreservesInv(k: Constants, s: Variables, s': Variables, dop: DiskOp)
+    requires Inv(k, s)
+    requires PageInResp(k, s, s', dop)
+    ensures Inv(k, s')
+  {
+    if (s'.Ready?) {
+      assert InvReady(k, s');
+    }
+  }
+
+  lemma PageInIndirectionTableReqStepPreservesInv(k: Constants, s: Variables, s': Variables, dop: DiskOp)
+    requires Inv(k, s)
+    requires PageInIndirectionTableReq(k, s, s', dop)
+    ensures Inv(k, s')
+  {
+    if (s'.Ready?) {
+      assert InvReady(k, s');
+    }
+  }
+
+  lemma PageInIndirectionTableRespStepPreservesInv(k: Constants, s: Variables, s': Variables, dop: DiskOp)
+    requires Inv(k, s)
+    requires PageInIndirectionTableResp(k, s, s', dop)
+    ensures Inv(k, s')
+  {
+    if (s'.Ready?) {
+      assert InvReady(k, s');
+    }
+  }
+
+  lemma EvictStepPreservesInv(k: Constants, s: Variables, s': Variables, dop: DiskOp, ref: Reference)
+    requires Inv(k, s)
+    requires Evict(k, s, s', dop, ref)
+    ensures Inv(k, s')
+  {
+    if (s'.Ready?) {
+      assert InvReady(k, s');
+    }
+  }
+
+  lemma NextStepPreservesInv(k: Constants, s: Variables, s': Variables, dop: DiskOp, step: Step)
+    requires Inv(k, s)
+    requires NextStep(k, s, s', dop, step)
+    ensures Inv(k, s')
+  {
+    match step {
+      case WriteBackReqStep(ref) => WriteBackReqStepPreservesInv(k, s, s', dop, ref);
+      case WriteBackRespStep => WriteBackRespStepPreservesInv(k, s, s', dop);
+      case WriteBackIndirectionTableReqStep => WriteBackIndirectionTableReqStepPreservesInv(k, s, s', dop);
+      case WriteBackIndirectionTableRespStep => WriteBackIndirectionTableRespStepPreservesInv(k, s, s', dop);
+      case UnallocStep(ref) => UnallocStepPreservesInv(k, s, s', dop, ref);
+      case PageInReqStep(ref) => PageInReqStepPreservesInv(k, s, s', dop, ref);
+      case PageInRespStep => PageInRespStepPreservesInv(k, s, s', dop);
+      case PageInIndirectionTableReqStep => PageInIndirectionTableReqStepPreservesInv(k, s, s', dop);
+      case PageInIndirectionTableRespStep => PageInIndirectionTableRespStepPreservesInv(k, s, s', dop);
+      case EvictStep(ref) => EvictStepPreservesInv(k, s, s', dop, ref);
+      case NoOpStep => { }
+      case TransactionStep(ops) => TransactionStepPreservesInv(k, s, s', dop, ops);
+    }
+  }
+
+  lemma NextPreservesInv(k: Constants, s: Variables, s': Variables, dop: DiskOp)
+    requires Inv(k, s)
+    requires Next(k, s, s', dop)
+    ensures Inv(k, s')
+  {
+    var step :| NextStep(k, s, s', dop, step);
+    NextStepPreservesInv(k, s, s', dop, step);
+  }
+
 }
 
